

$$2) a) \log \left[\frac{p(\ell_1 | x_n)}{p(\ell_2 | x_n)} \right] = \log \left[\frac{\frac{1}{S_1 \sqrt{2\pi}} \exp\left(-\frac{x_n - m_1}{2S_1^2}\right) \cdot \frac{N_1}{N_1 + N_2}}{\frac{1}{S_2 \sqrt{2\pi}} \exp\left(-\frac{x_n - m_2}{2S_2^2}\right) \cdot \frac{N_2}{N_1 + N_2}} \right]$$

$$0 = \log \left[\frac{S_2 \cdot N_1 \cdot \exp\left(\frac{x_n - m_2}{2S_2^2} - \frac{x_n - m_1}{2S_1^2}\right)}{S_1 \cdot N_2} \right]$$

$$1 = \frac{S_2 \cdot N_1}{S_1 \cdot N_2} \exp\left(\frac{S_1^2(x_n - m_2) - S_2^2(x_n - m_1)}{2S_2^2 S_1^2}\right)$$

$$\ln\left(\frac{S_1 N_2}{S_2 N_1}\right) = \frac{x_n(S_1^2 - S_2^2) - S_1^2 m_2 + S_2^2 m_1}{2S_2^2 S_1^2}$$

$$2S_2^2 S_1^2 \ln\left(\frac{S_1 N_2}{S_2 N_1}\right) + S_1^2 m_2 - S_2^2 m_1 = x_n(S_1^2 - S_2^2)$$

$$x_n = \frac{2S_2^2 S_1^2 \ln\left(\frac{S_1 N_2}{S_2 N_1}\right) + S_1^2 m_2 - S_2^2 m_1}{S_1^2 - S_2^2}$$

$$* x_n = \frac{2S_2^2 S_1^2 \ln\left(\frac{S_1 N_2}{S_2 N_1}\right) + S_1^2 m_2 - S_2^2 m_1}{S_1^2 - S_2^2}$$